compiler/dsl/coq/ReflexIO.v
@@ -1,7 +1,8 @@
-Require Import List.
 Require Import Ascii.
-Require Import String.
+Require Import Eqdep_dec.
+Require Import List.
 Require Import NPeano.
+Require Import String.
 Require Import Ynot.
 
 Open Scope char_scope.
@@ -10,6 +11,8 @@ Open Scope stsepi_scope.
 
 Require Import ReflexBase.
 Require Import ReflexDenoted.
+Require Import ReflexFin.
+Require Import ReflexHVec.
 Require Import ReflexVec.
 
 Ltac sep' := sep fail idtac.
@@ -30,10 +33,248 @@ Axiom traced : Trace -> hprop.
 
 Axiom open : fd -> hprop.
 
+Inductive desc : Set := num_d | str_d | fd_d.
+
+Definition desc_eqdec : forall x y : desc, decide (x = y).
+Proof.
+  decide equality.
+Qed.
+
+Module DecidableTypeDesc <: DecidableType.
+  Definition U := desc.
+  Definition eq_dec := desc_eqdec.
+End DecidableTypeDesc.
+
+Module DecidableEqDepDesc := DecidableEqDep(DecidableTypeDesc).
+
+Definition UIP_refl_desc :
+  forall (d : desc) (e : d = d), e = Logic.eq_refl d :=
+  DecidableEqDepDesc.UIP_refl.
+
+Fixpoint sdenote_desc (d : desc) : Set :=
+  match d with
+  | num_d => num
+  | str_d => str
+  | fd_d  => fd
+  end
+.
+
+Instance SDenoted_desc : SDenoted desc :=
+{ sdenote := sdenote_desc
+}.
+
+Axiom oracle : forall (d : desc) (tr : [Trace]), s[[ d ]].
+
 Axiom exec :
   forall (prog : str) (args : list str) (tr : [Trace]),
     STsep (tr ~~ traced tr)
-          (fun f : fd => tr ~~ open f * traced (Exec prog args f :: tr)).
+          (fun f : fd => [f = oracle fd_d tr]
+                         * (tr ~~ open f * traced (Exec prog args f :: tr))).
+(*
+Definition vdesc' n : Set := svec desc n.
+
+Definition sdenote_vdesc' n (pt : vdesc' n) : Set :=
+  shvec sdenote_desc pt.
+
+Instance SDenoted_vdesc' {n} : SDenoted (vdesc' n) :=
+{ sdenote := sdenote_vdesc' n
+}.
+
+(* Thank you Ynot for breaking sigT notation... *)
+Definition vdesc := (sigT (fun (n : nat) => vdesc' n)).
+
+Definition sdenote_vdesc (v : vdesc) : Set :=
+  sdenote_vdesc' (projT1 v) (projT2 v).
+
+Instance SDenoted_vdesc : SDenoted vdesc :=
+{ sdenote := sdenote_vdesc
+}.
+
+Definition vvdesc n := vec vdesc n.
+
+Section WITH_PAYLOAD_DESC_VEC.
+
+Context {NB_MSG : nat}.
+Variable VVD : vvdesc NB_MSG.
+
+Record compd :=
+{ compd_name : str
+; compd_cmd  : str
+; compd_args : list str
+; compd_conf : vdesc
+}.
+
+Variable COMPT : Set.
+
+Variable COMPTDEC : forall (x y : COMPT), decide (x = y).
+
+Variable COMPS : COMPT -> compd.
+
+Definition comp_conf_desc compt := compd_conf (COMPS compt).
+
+Record comp : Set :=
+{ comp_type : COMPT
+; comp_fd   : fd
+; comp_conf : s[[ comp_conf_desc comp_type ]]
+}.
+
+Inductive cdesc :=
+| Desc : desc -> cdesc
+| Comp : COMPT -> cdesc
+.
+
+Definition sdenote_cdesc cd :=
+  match cd with
+  | Desc d => sdenote_desc d
+  | Comp t => sigT (fun c : comp => comp_type c = t)
+  end.
+
+Instance SDenoted_cdesc : SDenoted cdesc :=
+{ sdenote := sdenote_cdesc
+}.
+
+Definition vcdesc' n : Set := svec cdesc n.
+
+Definition sdenote_vcdesc' n (pt : vcdesc' n) : Set :=
+  shvec sdenote_cdesc pt.
+
+Instance SDenoted_vcdesc' {n} : SDenoted (vcdesc' n) :=
+{ sdenote := sdenote_vcdesc' n
+}.
+
+Definition vcdesc := (sigT (fun (n : nat) => vcdesc' n)).
+
+Definition sdenote_vcdesc (v : vcdesc) : Set :=
+  sdenote_vcdesc' (projT1 v) (projT2 v).
+
+Instance SDenoted_vcdesc : SDenoted vcdesc :=
+{ sdenote := sdenote_vcdesc
+}.
+
+Fixpoint vdesc_to_vcdesc' {n : nat} : vdesc' n -> vcdesc' n :=
+  match n with
+  | O => fun _ => tt
+  | S n' => fun v =>
+    match v with (d, v') => (Desc d, vdesc_to_vcdesc' v') end
+  end.
+
+Fixpoint vdesc_to_vcdesc (v : vdesc) : vcdesc :=
+  match v with existT n v' => existT _ n (vdesc_to_vcdesc' v') end.
+
+Definition lkup_tag (tag : fin NB_MSG) : vdesc :=
+  vec_ith VVD tag.
+
+Record msg : Set :=
+  { tag : fin NB_MSG
+  ; pay : s[[ lkup_tag tag ]]
+  }.
+
+Record bogus_msg : Set :=
+  { btag : num
+  ; bbad : nat_of_num btag >= NB_MSG
+  }.
+
+Definition maybe_msg := (msg + bogus_msg)%type.
+
+Inductive KAction : Set :=
+| KExec   : str -> list str -> fd -> KAction
+| KCall   : str -> list str -> fd -> KAction
+| KSelect : list comp -> comp -> KAction
+| KSend   : comp -> msg -> KAction
+| KRecv   : comp -> msg -> KAction
+| KBogus  : comp -> bogus_msg -> KAction
+.
+
+Definition KTrace : Set :=
+  list KAction.
+
+Definition proj_fds : list comp -> list fd :=
+  map (fun comp => comp_fd comp).
+
+Definition trace_recv (f : fd) (d : desc) : s[[ d ]] -> Trace :=
+  match d with
+  | num_d => fun n : num => RecvNum f n
+  | str_d => fun s : str => RecvStr f s
+  | fd_d  => fun g : fd  => RecvFD  f g :: nil
+  end.
+
+Definition trace_send (f : fd) (d : desc) : s[[ d ]] -> Trace :=
+  match d with
+  | num_d => fun n : num => SendNum f n
+  | str_d => fun s : str => SendStr f s
+  | fd_d  => fun g : fd  => SendFD  f g :: nil
+  end.
+
+Section WITH_TRACE_FUN.
+
+Variable trace_fun : fd -> forall (d : desc), s[[ Desc d ]] -> list Action.
+
+Fixpoint trace_payload' (f : fd) (n : nat) :
+  forall (pd : vdesc' n) (p : s[[ pd ]]), Trace :=
+  match n with
+  | O => fun _ _ => nil
+  | S n' => fun pd =>
+    let (d, pd') as _pd return forall (p : sdenote_vdesc' (S n') _pd), _ := pd in
+    fun p => trace_payload' f n' pd' (snd p) ++ trace_fun f d (fst p)
+  end.
+
+Definition trace_payload (pd : vdesc) (f : fd) :=
+  trace_payload' f (projT1 pd) (projT2 pd).
+
+Definition trace_opt_payload (opd : option vdesc) (f : fd)
+  : s[! opd !] -> Trace :=
+  match opd as _opd return s[! _opd !] -> Trace with
+  | None => fun p => match p with end
+  | Some spt => fun p => trace_payload spt f p
+  end.
+
+End WITH_TRACE_FUN.
+
+Definition trace_payload_recv' := trace_payload' trace_recv.
+
+Definition trace_payload_send' := trace_payload' trace_send.
+
+Definition trace_payload_recv := trace_payload trace_recv.
+
+Definition trace_payload_send := trace_payload trace_send.
+
+Definition trace_opt_payload_recv := trace_opt_payload trace_recv.
+
+Definition trace_opt_payload_send := trace_opt_payload trace_send.
+
+Definition trace_recv_msg (f : fd) (m : msg) : Trace :=
+  let t := tag m in
+  trace_payload_recv (lkup_tag t) f (pay m) ++ RecvNum f (num_of_fin t).
+
+Definition trace_recv_bogus_msg (f : fd) (m : bogus_msg) : Trace :=
+  RecvNum f (btag m).
+
+Definition trace_recv_maybe_msg (f : fd) (m : maybe_msg) : Trace :=
+  match m with
+  | inl m => trace_recv_msg f m
+  | inr bm => trace_recv_bogus_msg f bm
+  end.
+
+Definition trace_send_msg (f : fd) (m : msg) : Trace :=
+  let t := tag m in
+  trace_payload_send (lkup_tag t) f (pay m) ++ SendNum f (num_of_fin t).
+
+Definition expand_kaction (ka : KAction) : Trace :=
+  match ka with
+  | KExec cmd args f => Exec cmd args f :: nil
+  | KCall cmd args pipe => Call cmd args pipe :: nil
+  | KSelect cs c => Select (proj_fds cs) (comp_fd c) :: nil
+  | KSend c m => trace_send_msg (comp_fd c) m
+  | KRecv c m => trace_recv_msg (comp_fd c) m
+  | KBogus c bm => trace_recv_bogus_msg (comp_fd c) bm
+  end.
+
+Fixpoint expand_ktrace (kt : KTrace) : Trace :=
+  match kt with
+  | nil => nil
+  | ka :: kas => expand_kaction ka ++ expand_ktrace kas
+  end.
+*)
 
 Axiom call :
   forall (prog : str) (args : list str) (tr : [Trace]),
